Simplified array interface with example proof

library/modelled.v
@@ -77,17 +77,17 @@ Proof.
   exact (@Isomorphism_dep_fn A A' (fun _ => B) (fun _ => B') i1 (fun _ _ _ => i2)).
 Defined.
 
-(* Check f_equal. *)
-
-(* Lemma Isomorphism_f_equal {A B : Type} (F : Type -> Type) : *)
-(*   Isomorphism A B -> Isomorphism (F A) (F B). *)
-(* Proof. *)
-(*   intros [f t ft tf]. *)
-(*   refine {| from := fun (a : F A) => _; to := _; from_to := _; to_from := _ |}. *)
-(*   econstructor. *)
-(*   instantiate (1 := ltac:()). *)
-
-
+Lemma Isomorphism_pair {A A' B B' : Type} :
+  Isomorphism A A' -> Isomorphism B B' -> Isomorphism (A * B) (A' * B').
+Proof.
+  intros [f1 t1 ft1 tf1] [f2 t2 ft2 tf2].
+  econstructor.
+  instantiate (1:= ltac:(intros [a b]; split; auto)).
+  instantiate (1:= ltac:(intros [a b]; split; auto)).
+  all: intros; intuition.
+  rewrite ft1, ft2; auto.
+  rewrite tf1, tf2; auto.
+Defined.
 
 Ltac eq_refl_match :=
   match goal with
@@ -208,14 +208,14 @@ Module FM <: UInt63.
    Qed.
 
   Definition add (x y: t) : t :=
-  let '(exist xz x_pf) := x in 
-  let '(exist yz y_pf) := y in 
+  let '(exist xz x_pf) := x in
+  let '(exist yz y_pf) := y in
   let z := ((xz + yz) mod (2^63))%Z in
   exist _ z (mod63_ok _).
 
   Definition mul (x y: t) : t :=
-  let '(exist xz x_pf) := x in 
-  let '(exist yz y_pf) := y in 
+  let '(exist xz x_pf) := x in
+  let '(exist yz y_pf) := y in
   let z := ((xz * yz) mod (2^63))%Z in
   exist _ z (mod63_ok _).
 
@@ -230,17 +230,6 @@ Module C : UInt63.
 End C.
 
 Module UInt63_Proofs.
-
-  Require Import JMeq.
-  (* Axiom P_pf : forall (T : Type) (P : (T -> FM.t) -> Prop) , *)
-  (*     (C.t = FM.t -> JMeq C.add FM.add -> JMeq C.mul FM.mul -> JMeq C.from_Z FM.from_Z -> JMeq C.to_Z FM.to_Z -> *)
-  (*      forall x x', (forall i, JMeq (x i) (x' i)) -> (P x = P x')). *)
-
-
-  (* Axiom P_pf : forall (T : Type) (P : (T -> C.t) -> Prop) (P' : (T -> FM.t) -> Prop), *)
-  (*     (C.t = FM.t -> JMeq C.add FM.add -> JMeq C.mul FM.mul -> JMeq C.from_Z FM.from_Z -> JMeq C.to_Z FM.to_Z -> *)
-  (*      forall x x', (forall i, JMeq (x i) (x' i)) -> (P x = P' x')). *)
-
 
   Definition Rep_Z : Rep Z. Admitted.
   Axiom Isomorphism_t : Isomorphism C.t FM.t.
@@ -376,86 +365,56 @@ End IntVerification.
 
 Module ArrayVerification.
 
-Module Type Element.
+Module Type ArraySetup.
   Axiom t : Type.
-End Element.
+  Axiom len: nat.
+  Axiom init : t.
+End ArraySetup.
 
-Module Type Array (E : Element).
-  Axiom arrays : Type.
-  Definition ST (S : Type) (A : Type) : Type := arrays -> A * arrays.
-  Axiom pure : forall {S A}, A -> ST S A.
-  Axiom bind : forall {S A B}, ST S A -> (A -> ST S B) -> ST S B.
-  Axiom runST : forall {A}, (forall S, ST S A) -> A.
-  Axiom array : Type -> Type.
-  Axiom new : forall {S}, nat -> E.t -> ST S (array S).
-  Axiom set : forall {S}, array S -> nat -> E.t -> ST S unit.
-  Axiom get : forall {S}, array S -> nat -> ST S (option E.t).
-  Axiom delete : forall {S}, array S -> ST S unit.
+Module Type Array (E : ArraySetup).
+  Axiom state : Type.
+  Definition M (A : Type) : Type := state -> A * state.
+  Axiom pure : forall {A}, A -> M A.
+  Axiom bind : forall {A B}, M A -> (A -> M B) -> M B.
+  Axiom runM : forall {A}, M A -> A.
+  Axiom set : nat -> E.t -> M unit.
+  Axiom get : nat -> M (option E.t).
 End Array.
 
-Module FM (E : Element) <: Array E.
-  Definition array (S : Type) : Type := nat.
-  Definition arrays := list (list E.t).
-  Definition ST (S : Type) (A : Type) : Type := arrays -> A * arrays.
-  Definition pure {S A} (a : A) : ST S A := fun s => (a, s).
-  Definition bind {S A B} (m : ST S A) (f : A -> ST S B) : ST S B :=
+(* Look at canon.replace_nth, invariants.replace_nth, sepalg_list.replace for lemmas *)
+Module FM (E : ArraySetup) <: Array E.
+  Definition state := list E.t.
+  Definition M (A : Type) : Type := state -> A * state.
+  Definition pure {A} (a : A) : M A := fun s => (a, s).
+  Definition bind {A B} (m : M A) (f : A -> M B) : M B :=
     fun s => f (fst (m s)) (snd (m s)).
     (* fun s => let '(a, s') := m s in f a s'. *)
-  Definition runST {A} (f : forall S, ST S A) : A :=
-    fst (f unit nil).
-  Definition new {S} (len : nat) (fill : E.t) : ST S (array S) :=
-    let xs := repeat fill len in
-    fun s => (length s, s ++ [xs]).
+  Definition runM {A} (m : M A) : A :=
+    fst (m (repeat E.init E.len)).
 
-  (* Look at canon.replace_nth, invariants.replace_nth, sepalg_list.replace for lemmas *)
-  Definition set {S} (arr : array S) (index : nat) (elt : E.t) : ST S unit :=
-    let fix replace (index : nat) (l : list E.t) : list E.t :=
-      match index, l with
-      | _, nil => nil
-      | O, cons x xs => cons elt xs
-      | S n, cons x xs => cons x (replace n xs)
-      end in
-    let fix aux (s : arrays) (arr : array S) : arrays :=
-      match arr, s with
-      | _, nil => nil
-      | O, cons x xs => cons (replace index x) xs
-      | S n, cons x xs => cons x (aux xs n)
-      end
-    in fun s => (tt, aux s arr).
+  Definition set (index : nat) (elt : E.t) : M unit :=
+    fun s => (tt, canon.replace_nth index s elt).
 
-  Definition get {S} (arr : array S) (index : nat) : ST S (option E.t) :=
-    fun s : arrays =>
-      match nth_error s arr with
-      | None => (None, s)
-      | Some l => (nth_error l index, s)
-      end.
+  Definition get (index : nat) : M (option E.t) :=
+    fun s => (nth_error s index, s).
 
-  Definition delete {S} (arr : array S) : ST S unit :=
-    let fix aux (s : arrays) (arr : array S) : arrays :=
-      match arr, s with
-      | _, nil => nil
-      | O, cons x xs => cons nil xs
-      | S n, cons x xs => cons x (aux xs n)
-      end
-    in fun s => (tt, aux s arr).
 End FM.
 
-Module C (E : Element) : Array E.
-  Axiom arrays : Type.
-  Definition ST (S : Type) (A : Type) : Type := arrays -> A * arrays.
-  Axiom pure : forall {S A}, A -> ST S A.
-  Axiom bind : forall {S A B}, ST S A -> (A -> ST S B) -> ST S B.
-  Axiom runST : forall {A}, (forall S, ST S A) -> A.
-  Axiom array : Type -> Type.
-  Axiom new : forall {S}, nat -> E.t -> ST S (array S).
-  Axiom set : forall {S}, array S -> nat -> E.t -> ST S unit.
-  Axiom get : forall {S}, array S -> nat -> ST S (option E.t).
-  Axiom delete : forall {S}, array S -> ST S unit.
+Module C (E : ArraySetup) : Array E.
+  Axiom state : Type.
+  Definition M (A : Type) : Type := state -> A * state.
+  Axiom pure : forall {A}, A -> M A.
+  Axiom bind : forall {A B}, M A -> (A -> M B) -> M B.
+  Axiom runM : forall {A}, M A -> A.
+  Axiom set : nat -> E.t -> M unit.
+  Axiom get : nat -> M (option E.t).
 End C.
 
 Module Array_Proofs.
   Module E.
     Definition t := bool.
+    Definition len := 5.
+    Definition init := false.
   End E.
   Module FM := FM E.
   Module C := C E.
@@ -463,80 +422,52 @@ Module Array_Proofs.
   Definition Rep_nat : Rep nat. Admitted.
   Definition Rep_t : Rep E.t. Admitted.
 
-  Variable Isomorphism_array : forall {S}, Isomorphism (C.array S) (FM.array S).
-  Variable Isomorphism_arrays : Isomorphism (C.arrays) (FM.arrays).
+  Axiom Isomorphism_state : Isomorphism C.state FM.state.
 
-  Definition Isomorphism_ST
-             {S A A' : Type} (I : Isomorphism A A') : Isomorphism (C.ST S A) (FM.ST S A').
-    destruct I as [f t pf pt].
-    destruct (@Isomorphism_array S) as [f' t' pf' pt'].
-    unfold FM.ST, C.ST.
-    apply Isomorphism_fn.
-    apply Isomorphism_arrays.
-    Admitted.
-
-
-
-
-
-  (* Axiom Isomorphism_ST : forall {S A A'}, Isomorphism A A' -> Isomorphism (C.ST S A) (FM.ST S A'). *)
-  Axiom Isomorphism_ST_inj : forall {S A A'}, Isomorphism (C.ST S A) (FM.ST S A') -> Isomorphism A A'.
+  Definition Isomorphism_M
+             {A A' : Type} (I : Isomorphism A A')
+             : Isomorphism (C.M A) (FM.M A').
+  Proof.
+    eauto using Isomorphism_fn, Isomorphism_state, Isomorphism_pair.
+  Qed.
 
   Definition pure_ep : extern_properties :=
     {| type_desc :=
-      @TYPEPARAM (fun (S : Type) `{Rep_S : Rep S} =>
         @TYPEPARAM (fun (A : Type) `{Rep_A : Rep A} =>
           @TRANSPARENT A Rep_A (Some (fun arr =>
-            @OPAQUE (C.ST S A) (FM.ST S A) (Isomorphism_ST _) None))))
+            @OPAQUE (C.M A) (FM.M A) (Isomorphism_M _) None)))
      ; prim_fn := @C.pure
      ; model_fn := @FM.pure
-     ; c_name := "st_pure"
+     ; c_name := "m_pure"
      |}.
 
   Definition bind_ep : extern_properties :=
     {| type_desc :=
-      @TYPEPARAM (fun (S : Type) `{Rep_S : Rep S} =>
         @TYPEPARAM (fun (A : Type) `{Rep_A : Rep A} =>
           @TYPEPARAM (fun (B : Type) `{Rep_B : Rep B} =>
-            @OPAQUE (C.ST S A) (FM.ST S A) (Isomorphism_ST _) (Some (fun m =>
-              @OPAQUE (A -> C.ST S B) (A -> FM.ST S B) (Isomorphism_fn _ (Isomorphism_ST _)) (Some (fun f =>
-                @OPAQUE (C.ST S B) (FM.ST S B) (Isomorphism_ST _) None)))))))
+            @OPAQUE (C.M A) (FM.M A) (Isomorphism_M _) (Some (fun m =>
+              @OPAQUE (A -> C.M B) (A -> FM.M B) (Isomorphism_fn _ (Isomorphism_M _)) (Some (fun f =>
+                @OPAQUE (C.M B) (FM.M B) (Isomorphism_M _) None))))))
      ; prim_fn := @C.bind
      ; model_fn := @FM.bind
-     ; c_name := "st_bind"
+     ; c_name := "m_bind"
      |}.
 
-  Definition runST_ep : extern_properties :=
+  Definition runM_ep : extern_properties :=
     {| type_desc :=
-      @TYPEPARAM (fun (A : Type) `{Rep_A : Rep A} =>
-          @OPAQUE (forall (S : Type), C.ST S A) (forall (S : Type), FM.ST S A)
-                  (@Isomorphism_dep_fn Type Type (fun S => C.ST S A) (fun S => FM.ST S A) _
-                                    (fun s s' m => @Isomorphism_ST _ A A _)) (Some (fun f =>
-            @TRANSPARENT A Rep_A None)))
-     ; prim_fn := @C.runST
-     ; model_fn := @FM.runST
-     ; c_name := "st_runST"
-     |}.
-
-  Definition new_ep : extern_properties :=
-    {| type_desc :=
-      @TYPEPARAM (fun (S : Type) `{Rep_S : Rep S} =>
-        @TRANSPARENT nat Rep_nat (Some (fun n =>
-          @TRANSPARENT E.t Rep_t (Some (fun a =>
-            @OPAQUE (C.ST S (C.array S)) (FM.ST S (FM.array S))
-                    (Isomorphism_ST Isomorphism_array) None)))))
-     ; prim_fn := @C.new
-     ; model_fn := @FM.new
-     ; c_name := "array_new"
+        @TYPEPARAM (fun (A : Type) `{Rep_A : Rep A} =>
+          @OPAQUE (C.M A) (FM.M A) (Isomorphism_M _)
+                  (Some (fun f => @TRANSPARENT A Rep_A None)))
+     ; prim_fn := @C.runM
+     ; model_fn := @FM.runM
+     ; c_name := "m_runM"
      |}.
 
   Definition set_ep : extern_properties :=
     {| type_desc :=
-      @TYPEPARAM (fun (S : Type) `{Rep_S : Rep S} =>
-        @OPAQUE (C.array S) (FM.array S) Isomorphism_array (Some (fun arr =>
-          @TRANSPARENT nat Rep_nat (Some (fun n =>
-            @TRANSPARENT E.t Rep_t (Some (fun a =>
-              @OPAQUE (C.ST S unit) (FM.ST S unit) (Isomorphism_ST _) None)))))))
+        @TRANSPARENT nat Rep_nat (Some (fun n =>
+          @TRANSPARENT E.t Rep_t (Some (fun a =>
+            @OPAQUE (C.M unit) (FM.M unit) (Isomorphism_M _) None))))
      ; prim_fn := @C.set
      ; model_fn := @FM.set
      ; c_name := "array_set"
@@ -544,946 +475,55 @@ Module Array_Proofs.
 
   Definition get_ep : extern_properties :=
     {| type_desc :=
-      @TYPEPARAM (fun (S : Type) `{Rep_S : Rep S} =>
-        @OPAQUE (C.array S) (FM.array S) Isomorphism_array (Some (fun arr =>
-          @TRANSPARENT nat Rep_nat (Some (fun n =>
-            @OPAQUE (C.ST S (option E.t)) (FM.ST S (option E.t)) (Isomorphism_ST _) None)))))
+        @TRANSPARENT nat Rep_nat (Some (fun n =>
+          @OPAQUE (C.M (option E.t)) (FM.M (option E.t)) (Isomorphism_M _) None))
      ; prim_fn := @C.get
      ; model_fn := @FM.get
      ; c_name := "array_get"
      |}.
 
-  Definition delete_ep : extern_properties :=
-    {| type_desc :=
-      @TYPEPARAM (fun (S : Type) `{Rep_S : Rep S} =>
-        @OPAQUE (C.array S) (FM.array S) Isomorphism_array (Some (fun arr =>
-          @OPAQUE (C.ST S unit) (FM.ST S unit) (Isomorphism_ST _) None)))
-     ; prim_fn := @C.delete
-     ; model_fn := @FM.delete
-     ; c_name := "array_delete"
-     |}.
-
   Axiom pure_properties : model_spec pure_ep.
   Axiom bind_properties : model_spec bind_ep.
-  Axiom runST_properties : model_spec runST_ep.
-  Axiom new_properties : model_spec new_ep.
+  Axiom runM_properties : model_spec runM_ep.
   Axiom set_properties : model_spec set_ep.
   Axiom get_properties : model_spec get_ep.
-  Axiom delete_properties : model_spec delete_ep.
 
   Ltac prim_rewrites :=
     repeat eq_refl_match;
     rewrite ?from_to, ?to_from.
 
-  (* Definition actions_equiv {S A : Type} (x y : FM.ST S A) : Prop := *)
-  (*   forall s, x s = y s. *)
-  (* Set Printing All. *)
-  (* Print actions_equiv. *)
-
-  (* Axiom runST_equiv : forall A (x y : forall (S : Type), FM.ST S A), *)
-  (*     x = y -> *)
-  (*     FM.runST x = FM.runST y. *)
-
-
   Arguments from A B {_}.
   Arguments to A B {_}.
 
-  Axiom array_eq : forall S, C.array S = FM.array S.
-  (* Lemma from_eq : *)
-  (*   forall A B x, *)
-  (*     A = B -> *)
-  (*     from A B x = x. *)
-
-  Lemma Isomorphism_FMST {A B : Type} : Isomorphism A B -> Isomorphism (FM.ST unit A) (FM.ST unit B).
-  Proof.
-    intros [f t ft tf].
-    econstructor.
-    Unshelve.
-    3: { intros a x. specialize (a x).
-         exact (f (fst a), (snd a)). }
-    3: { intros a x. specialize (a x).
-         exact (t (fst a), (snd a)). }
-    simpl. intros. apply functional_extensionality. intros. rewrite ?ft, ?tf. destruct (x x0). auto.
-    simpl. intros. apply functional_extensionality. intros. rewrite ?ft, ?tf. destruct (x x0). auto.
-  Defined.
-
-
-  (* Lemma from_eq : *)
-  (*   forall A B x, *)
-  (*     A = B -> *)
-  (*     forall (I1 : Isomorphism A B) (I2 : Isomorphism (FM.ST unit B) (FM.ST unit A)), *)
-  (*       I2 = Isomorphism_sym (Isomorphism_FMST I1) -> *)
-  (*   (@from A B I1 (fst (@from (FM.ST unit B) (FM.ST unit A) I2 x []))) = fst (x []). *)
-  (* Proof. *)
-  (*   intros A B X eq I1 I2 Ieq. *)
-  (*   subst. *)
-  (* Admitted. *)
-  (*   unfold fst. *)
-  (*   unfold fst. *)
-  (* Abort. *)
-
-  Require Import JMeq.
-
-  Require Import Coq.Logic.FunctionalExtensionality.
-  Require Import Coq.Logic.JMeq.
-
-  Theorem jmeq_funext
-    A (P : A -> Type) (Q : A -> Type)
-    (f : forall a, P a)(g : forall a, Q a)
-    (h : forall a, JMeq (f a) (g a)) : JMeq f g.
-  Proof.
-    assert (pq_eq : P = Q).
-      apply functional_extensionality.
-      exact (fun a => match (h a) with JMeq_refl => eq_refl end).
-    induction pq_eq.
-    assert (fg_eq : f = g).
-      apply functional_extensionality_dep.
-      exact (fun a => JMeq_rect (fun ga => f a = ga) eq_refl (h a)).
-    induction fg_eq.
-    exact JMeq_refl.
-  Qed.
-
-
-  Axiom runST_pf : forall {A : Type}
-                          {f : forall (S : Type), C.ST S A}
-                          {f' : forall (S : Type), FM.ST S A},
-   (forall (eq_array : forall {S}, (C.array S) = (FM.array S))
-           (eq_arrays : C.arrays = FM.arrays), JMeq f f') ->
-   (C.runST f) = (FM.runST f').
-
   Lemma set_get :
-    forall {S : Type} (n len : nat) (bound : n < len) (to_set to_fill : E.t),
-      (C.runST (fun _ => C.bind (C.new len to_fill) (fun arr => C.bind (C.set arr n to_set) (fun _ => C.get arr n))))
+    forall (n : nat) (bound : n < E.len) (to_set : E.t),
+      (C.runM (C.bind (C.set n to_set) (fun _ => C.get n)))
         =
-      (C.runST (fun _ => C.pure (Some to_set))).
+      (C.runM (C.pure (Some to_set))).
   Proof.
+    intros n bound to_set.
 
-    (* Set Printing Implicit. *)
-    (* Unset Printing Notations. *)
-
-
-    intros S n len bound to_set to_fill.
-(*
-
-    erewrite runST_pf.
-    instantiate (1 := fun _ => FM.bind (FM.new len to_fill) (fun arr => FM.bind (FM.set arr n to_set) (fun _ => FM.get arr n))).
-    erewrite runST_pf.
-    instantiate (1 := (fun _ => FM.pure (Some to_set))).
-
-
-    admit.
-
-
-    intros array_eq arrays_eq.
-    apply jmeq_funext.
-    intro A.
-    admit.
-
-    intros array_eq arrays_eq.
-    apply jmeq_funext.
-    intro A.
-    admit.
-*)
-    props runST_properties.
+    props runM_properties.
     prim_rewrites.
-    unfold FM.runST.
+    unfold FM.runM.
 
     props bind_properties.
     props pure_properties.
-    props new_properties.
     unfold FM.bind, FM.pure.
     prim_rewrites.
 
-    props bind_properties.
-    unfold FM.bind.
-    prim_rewrites.
-
     props set_properties.
-    prim_rewrites.
-
     props get_properties.
     prim_rewrites.
 
-    unfold fst at 4.
-
-    rewrite !to_sym.
-    rewrite !from_trans.
-(*
-    rewrite from_eq.
-    3: {
-      Set Printing All.
-      Check (@Isomorphism_ST unit (C.array unit) (C.array unit) (@Isomorphism_refl (C.array unit))).
-      unfold Isomorphism_sym.
-      simpl.
-      Set Printing All.
-      Check (@Isomorphism_ST unit (C.array unit) (C.array unit) (@Isomorphism_refl (C.array unit))).
-      Check (@Isomorphism_refl (FM.ST unit (FM.array unit))).
-      replace (@Isomorphism_ST unit (C.array unit) (C.array unit) (@Isomorphism_refl (C.array unit)))
-         with (@Isomorphism_refl (FM.ST unit (FM.array unit))).
-
-    }
-
-
-
-    Set Printing All.
-
-    (* rewrite array_eq. *)
-
-    (* Set Printing Implicit. *)
-
-    unfold FM.new, FM.set, FM.get.
-    unfold repeat.
-
-    simpl.
-    all: try auto.
-
-
-    rewrite !to_sym.
-    rewrite !from_trans.
-
-
-
-    Unset Printing Implicit.
-
-
-    (* rest of the proof is just about the functional model *)
-    Set Printing All.
-    Check (@FM.new unit len to_fill).
-    rewrite ?from_to, ?to_from.
-    unfold FM.new.
-    rewrite ?from_to, ?to_from.
-
-    unfold from.
-
-    assert (forall (x : FM.ST S nat), to (from x) = x).
-    intros. prim_rewrites. auto.
-
-
-    rewrite (H (fun s : FM.arrays => (length s, s ++ [repeat to_fill len]))).
-    rewrite !to_from.
-    unfold FM.get, FM.set, FM.new.
-    simpl.
-    prim_rewrites.
-*)
-  Admitted.
-
-End Array_Proofs.
-
-End ArrayVerification.
-Require Import String.
-
-Require Import ZArith.
-Require Import Psatz.
-Require Import List.
-Import ListNotations.
-
-
-Require Import Coq.Logic.FinFun.
-Require Import Coq.Relations.Relation_Definitions.
-Require Import Coq.Relations.Relation_Operators.
-Require Import Coq.Program.Basics.
-Require Import Coq.Program.Combinators.
-Require Import Setoid.
-
-(*
-Inductive P {A : Type} : A -> Prop :=
-| MkP : forall a, P a.
-
-Class Isomorphism (A B : Type) : Type :=
-  { from : A -> B
-  ; to : B -> A
-  ; from_to : forall (x : A), to (from x) = x
-  ; to_from : forall (x : B), from (to x) = x
-  }.
-
-(* Require Import Coq.Logic.FinFun. *)
-(* Require Import Coq.Relations.Relation_Definitions. *)
-(* Require Import Coq.Relations.Relation_Operators. *)
-(* Require Import Coq.Program.Basics. *)
-(* Require Import Coq.Program.Combinators. *)
-(* Require Import Setoid. *)
-
-Instance Isomorphism_refl {A : Type} : Isomorphism A A.
-Proof.
-  eapply {| from := id ; to := id ; from_to := ltac:(auto) ; to_from := ltac:(auto) |}.
-Defined.
-
-Lemma Isomorphism_sym {A B : Type} `(I : Isomorphism A B) : Isomorphism B A.
-Proof.
-  destruct I as [f t ft tf].
-  eapply {| from := t ; to := f ; from_to := tf ; to_from := ft |}.
-Defined.
-
-Lemma Isomorphism_trans {A B C : Type}
-      `(I1 : Isomorphism A B)
-      `(I2 : Isomorphism B C) : Isomorphism A C.
-Proof.
-  destruct I1 as [f1 t1 ft1 tf1].
-  destruct I2 as [f2 t2 ft2 tf2].
-  eapply {| from := fun x => f2 (f1 x)
-          ; to := fun x => t1 (t2 x)
-          ; from_to := _
-          ; to_from := _|}.
-
-  Unshelve.
-  intros; simpl; rewrite ft2, ft1; auto.
-  intros; simpl; rewrite tf1, tf2; auto.
-Defined.
-
-Lemma from_sym : forall A B `(M : Isomorphism A B),
-    @from A B M = @to B A (Isomorphism_sym M).
-Proof.
-  intros A B M; destruct M; auto.
-Defined.
-
-Lemma to_sym : forall A B `(M : Isomorphism A B),
-    @to A B M = @from B A (Isomorphism_sym M).
-Proof.
-  intros A B M; destruct M; auto.
-Defined.
-
-Lemma from_trans : forall A B C `(M1 : Isomorphism A B) `(M2 : Isomorphism B C),
-    forall (x : A), @from B C M2 (@from A B M1 x) = @from A C (Isomorphism_trans M1 M2) x .
-Proof.
-  intros A B C [f1 t1 pf1 pt1] [f2 t2 pf2 pt2] x; simpl; auto.
-Defined.
-
-
-Require Import Coq.Logic.FunctionalExtensionality.
-
-Lemma Isomorphism_dep_fn {A A' : Type} {B : A -> Type} {B' : A' -> Type} :
-  Isomorphism A A' ->
-  (forall (a : A) (a' : A'), Isomorphism A A' -> Isomorphism (B a) (B' a')) ->
-  Isomorphism (forall (a : A), B a) (forall (a' : A'), B' a').
-Proof.
-  intros.
-  econstructor.
-  instantiate (1 := ltac:(intros g a; exact (from (g (to a))))).
-  instantiate (1 := ltac:(intros g a'; exact (to (g (from a'))))).
-  all: intros; apply functional_extensionality_dep;
-       intro; rewrite ?from_to, ?to_from; auto.
-Defined.
-
-Lemma Isomorphism_fn {A A' B B' : Type} :
-  Isomorphism A A' -> Isomorphism B B' -> Isomorphism (A -> B) (A' -> B').
-Proof.
-  intros i1 i2.
-  exact (@Isomorphism_dep_fn A A' (fun _ => B) (fun _ => B') i1 (fun _ _ _ => i2)).
-Defined.
-
-Check f_equal.
-
-(* Lemma Isomorphism_f_equal {A B : Type} (F : Type -> Type) : *)
-(*   Isomorphism A B -> Isomorphism (F A) (F B). *)
-(* Proof. *)
-(*   intros [f t ft tf]. *)
-(*   refine {| from := fun (a : F A) => _; to := _; from_to := _; to_from := _ |}. *)
-(*   econstructor. *)
-(*   instantiate (1 := ltac:()). *)
-
-
-
-Ltac eq_refl_match :=
-  match goal with
-  | [ |- context[match ?x with | eq_refl => _ end] ] => destruct x
-  (* | [ _ : context[match ?x with | eq_refl => _ end] |- _] => destruct x *)
-  end.
-
-Ltac props x :=
-  let P := fresh in
-  pose proof x as P;
-  hnf in P;
-  simpl in P;
-  rewrite !P;
-  unfold id, eq_rect in *;
-  clear P.
-
-Require Import VeriFFI.library.meta.
-
-(* opaque and transparent *)
-Inductive annotated : Type :=
-| TYPEPARAM : (forall (A : Type) `{Rep A}, annotated) -> annotated
-| OPAQUE : forall (prim_type model_type : Type)
-                    `{Isomorphism prim_type model_type},
-                    (option (prim_type -> annotated)) ->
-                    annotated
-| TRANSPARENT : forall (A : Type) `{Rep A}, (option (A -> annotated)) -> annotated.
-
-Definition Rep_Z : Rep Z. Admitted.
-
-Theorem Rep_any : forall {A : Type}, Rep A. Admitted.
-
-Fixpoint to_prim_fn_type (r : annotated) : Type :=
-  match r with
-  | TYPEPARAM f => forall (A : Type), to_prim_fn_type (f A Rep_any)
-  | OPAQUE pt mt M o =>
-      match o with
-      | None => pt
-      | Some fp => forall (p : pt), to_prim_fn_type (fp p)
-      end
-  | TRANSPARENT t R o =>
-      match o with
-      | None => t
-      | Some f => forall (x : t), to_prim_fn_type (f x)
-      end
-  end.
-
-Fixpoint to_model_fn_type (r : annotated) : Type :=
-  match r with
-  | TYPEPARAM f => forall (A : Type), to_model_fn_type (f A Rep_any)
-  | OPAQUE pt mt M o =>
-      match o with
-      | None => mt
-      | Some fp => forall (m : mt), to_model_fn_type (fp (@to pt mt M m))
-      end
-  | TRANSPARENT t R o =>
-      match o with
-      | None => t
-      | Some f => forall (x : t), to_model_fn_type (f x)
-      end
-  end.
-
-Record extern_properties :=
-  { type_desc : annotated
-  ; prim_fn : to_prim_fn_type type_desc
-  ; model_fn : to_model_fn_type type_desc
-  ; c_name : string
-  }.
-
-Fixpoint model_spec_aux
-         (a : annotated)
-         (ft : to_prim_fn_type a)
-         (mt : to_model_fn_type a) {struct a} : Prop.
-destruct a as [f|prim_type model_type M|A R o]; simpl in ft, mt.
-* exact (forall (A : Type), model_spec_aux (f A Rep_any) (ft A) (mt A)).
-* destruct o as [pf|].
-  - refine (forall (x : prim_type), model_spec_aux (pf x) (ft x) _).
-    pose (m := mt (@from prim_type model_type M x)).
-    rewrite from_to in m.
-    exact m.
-  - exact (ft = to mt).
-* destruct o as [pf|].
-  - exact (forall (x : A), model_spec_aux (pf x) (ft x) (mt x)).
-  - exact (ft = mt).
-Defined.
-
-Definition model_spec (ep : extern_properties) : Prop :=
-  model_spec_aux (type_desc ep) (prim_fn ep) (model_fn ep).
-
-Module IntVerification.
-
-Module Type UInt63.
-  Axiom t : Type.
-  Axiom from_Z : Z -> t.
-  Axiom to_Z : t -> Z.
-  Axiom add : t -> t -> t.
-  Axiom mul : t -> t -> t.
-End UInt63.
-
-(* Axiom VSU : Type. *)
-(* Axiom int63_vsu : VSU. *)
-(* Axiom lift : forall {A : Type}, A -> VSU -> string -> A. *)
-
-Module FM <: UInt63.
-  Definition t := {z : Z | 0 <= z < 2^63}%Z.
-  Definition from_Z (z : Z) : t.
-    exists (Z.modulo z (2^63)).
-    apply Z_mod_lt.
-    constructor.
-  Defined.
-
-  Definition to_Z (z : t) : Z := proj1_sig z.
-  Definition add (x y : t) : t.
-    destruct x as [xz x_pf], y as [yz y_pf].
-    exists ((xz + yz) mod (2^63))%Z.
-    split.
-    * destruct x_pf as [x_pf1 _], y_pf as [y_pf1 _].
-      apply Z_mod_nonneg_nonneg.
-      apply Z.add_nonneg_nonneg.
-      assumption. assumption.
-      apply Pos2Z.is_nonneg.
-    * apply Z.mod_pos_bound.
-      constructor.
-  Defined.
-
-  Definition mul (x y : t) : t.
-    destruct x as [xz x_pf], y as [yz y_pf].
-    exists ((xz * yz) mod (2^63))%Z.
-    split.
-    * destruct x_pf as [x_pf1 _], y_pf as [y_pf1 _].
-      apply Z_mod_nonneg_nonneg.
-      apply Z.mul_nonneg_nonneg.
-      assumption. assumption.
-      apply Pos2Z.is_nonneg.
-    * apply Z.mod_pos_bound.
-      constructor.
-  Defined.
-End FM.
-
-Module C : UInt63.
-  Axiom t : Type.
-  Axiom from_Z : Z -> t.
-  Axiom to_Z : t -> Z.
-  Axiom add : t -> t -> t.
-  Axiom mul : t -> t -> t.
-End C.
-
-Module UInt63_Proofs.
-  Definition Rep_Z : Rep Z. Admitted.
-  Axiom Isomorphism_t : Isomorphism C.t FM.t.
-
-  Definition from_Z_ep : extern_properties :=
-    {| type_desc :=
-        @TRANSPARENT Z Rep_Z
-           (Some (fun z => @OPAQUE _ _ Isomorphism_t None))
-     ; prim_fn := C.from_Z
-     ; model_fn := FM.from_Z
-     ; c_name := "int63_from_Z"
-     |}.
-
-  Definition to_Z_ep : extern_properties :=
-    {| type_desc :=
-        @OPAQUE _ _ Isomorphism_t
-           (Some (fun z => @TRANSPARENT Z Rep_Z None))
-     ; prim_fn := C.to_Z
-     ; model_fn := FM.to_Z
-     ; c_name := "int63_to_Z"
-     |}.
-
-  Definition add_ep : extern_properties :=
-    {| type_desc :=
-          @OPAQUE _ _ Isomorphism_t
-            (Some (fun i =>
-              @OPAQUE _ _ Isomorphism_t
-                (Some (fun i => @OPAQUE _ _ Isomorphism_t None))))
-     ; prim_fn := C.add
-     ; model_fn := FM.add
-     ; c_name := "int63_add"
-     |}.
-
-  Definition mul_ep : extern_properties :=
-    {| type_desc :=
-          @OPAQUE _ _ Isomorphism_t
-            (Some (fun i =>
-              @OPAQUE _ _ Isomorphism_t
-                (Some (fun i => @OPAQUE _ _ Isomorphism_t None))))
-     ; prim_fn := C.mul
-     ; model_fn := FM.mul
-     ; c_name := "int63_mul"
-     |}.
-
-  Axiom from_Z_properties : model_spec from_Z_ep.
-  Axiom to_Z_properties : model_spec to_Z_ep.
-  Axiom add_properties : model_spec add_ep.
-  Axiom mul_properties : model_spec mul_ep.
-
-  Lemma seven : C.to_Z (C.add (C.from_Z 3%Z) (C.from_Z 4%Z)) = 7%Z.
-  Proof.
-    props from_Z_properties.
-    props to_Z_properties.
-    props add_properties.
-    repeat eq_refl_match.
-    rewrite !from_to, !to_from.
-    unfold FM.to_Z, FM.add, FM.from_Z.
-    simpl.
-    rewrite Z.mod_small.
-    auto.
+    unfold fst at 2.
+
+    (* unfold FM.get, FM.set in *. *)
+    eapply canon.nth_error_replace_nth.
+    apply nth_error_repeat.
     lia.
   Qed.
 
-  Lemma add_assoc : forall (x y z : Z),
-    C.to_Z (C.add (C.from_Z x) (C.add (C.from_Z y) (C.from_Z z))) =
-    C.to_Z (C.add (C.add (C.from_Z x) (C.from_Z y)) (C.from_Z z)).
-  Proof.
-    intros x y z.
-    props from_Z_properties.
-    props to_Z_properties.
-    props add_properties.
-    repeat eq_refl_match.
-    rewrite !from_to, !to_from.
-    unfold FM.add, FM.from_Z, FM.to_Z.
-    simpl.
-    rewrite <- !(Z.add_mod y z).
-    rewrite <- !(Z.add_mod x y).
-    rewrite <- !(Z.add_mod).
-    f_equal.
-    apply Z.add_assoc.
-    all: lia.
-  Qed.
-
-  Lemma mul_add_distr_l : forall (x y z : Z),
-    C.to_Z (C.mul (C.from_Z x) (C.add (C.from_Z y) (C.from_Z z))) =
-    C.to_Z (C.add (C.mul (C.from_Z x) (C.from_Z y)) (C.mul (C.from_Z x) (C.from_Z z))).
-  Proof.
-    intros x y z.
-    props from_Z_properties.
-    props to_Z_properties.
-    props add_properties.
-    props mul_properties.
-    repeat eq_refl_match.
-    rewrite !from_to, !to_from.
-    unfold FM.mul, FM.add, FM.from_Z, FM.to_Z.
-    simpl.
-    pose (y' := Z.modulo y (Z.pow_pos 2 63)); fold y'.
-    pose (z' := Z.modulo z (Z.pow_pos 2 63)); fold z'.
-    rewrite <- Zplus_mod.
-    rewrite <- Z.mul_add_distr_l.
-    rewrite Zmult_mod_idemp_r.
-    auto.
-  Qed.
-
-  Lemma mul_add_distr_r : forall (x y z : Z),
-    C.to_Z (C.mul (C.add (C.from_Z x) (C.from_Z y)) (C.from_Z z)) =
-    C.to_Z (C.add (C.mul (C.from_Z x) (C.from_Z z)) (C.mul (C.from_Z y) (C.from_Z z))).
-  Proof.
-    intros x y z.
-    props from_Z_properties.
-    props to_Z_properties.
-    props add_properties.
-    props mul_properties.
-    repeat eq_refl_match.
-    rewrite !from_to, !to_from.
-    unfold FM.mul, FM.add, FM.from_Z, FM.to_Z.
-    simpl.
-    pose (x' := Z.modulo y (Z.pow_pos 2 63)); fold x'.
-    pose (y' := Z.modulo y (Z.pow_pos 2 63)); fold y'.
-    pose (z' := Z.modulo z (Z.pow_pos 2 63)); fold z'.
-    rewrite <- Zplus_mod.
-    rewrite <- Z.mul_add_distr_r.
-    rewrite Zmult_mod_idemp_l.
-    auto.
-  Qed.
-
-End UInt63_Proofs.
-
-End IntVerification.
-
-Module ArrayVerification.
-
-Module Type Element.
-  Axiom t : Type.
-End Element.
-
-Module Type Array (E : Element).
-  Axiom ST : Type -> Type -> Type.
-  Axiom pure : forall {S A}, A -> ST S A.
-  Axiom bind : forall {S A B}, ST S A -> (A -> ST S B) -> ST S B.
-  Axiom runST : forall {A}, (forall S, ST S A) -> A.
-  Axiom array : Type -> Type.
-  Axiom new : forall {S}, nat -> E.t -> ST S (array S).
-  Axiom set : forall {S}, array S -> nat -> E.t -> ST S unit.
-  Axiom get : forall {S}, array S -> nat -> ST S (option E.t).
-  Axiom delete : forall {S}, array S -> ST S unit.
-End Array.
-
-Module FM (E : Element) <: Array E.
-  Definition array (S : Type) : Type := nat.
-  Definition arrays := list (list E.t).
-  Definition ST (S : Type) (A : Type) : Type := arrays -> A * arrays.
-  Definition pure {S A} (a : A) : ST S A := fun s => (a, s).
-  Definition bind {S A B} (m : ST S A) (f : A -> ST S B) : ST S B :=
-    fun s => f (fst (m s)) (snd (m s)).
-    (* fun s => let '(a, s') := m s in f a s'. *)
-  Definition runST {A} (f : forall S, ST S A) : A :=
-    fst (f unit nil).
-  Definition new {S} (len : nat) (fill : E.t) : ST S (array S) :=
-    let xs := repeat fill len in
-    fun s => (length s, s ++ [xs]).
-
-  (* Look at canon.replace_nth, invariants.replace_nth, sepalg_list.replace for lemmas *)
-  Definition set {S} (arr : array S) (index : nat) (elt : E.t) : ST S unit :=
-    let fix replace (index : nat) (l : list E.t) : list E.t :=
-      match index, l with
-      | _, nil => nil
-      | O, cons x xs => cons elt xs
-      | S n, cons x xs => cons x (replace n xs)
-      end in
-    let fix aux (s : arrays) (arr : array S) : arrays :=
-      match arr, s with
-      | _, nil => nil
-      | O, cons x xs => cons (replace index x) xs
-      | S n, cons x xs => cons x (aux xs n)
-      end
-    in fun s => (tt, aux s arr).
-
-  Definition get {S} (arr : array S) (index : nat) : ST S (option E.t) :=
-    fun s : arrays =>
-      match nth_error s arr with
-      | None => (None, s)
-      | Some l => (nth_error l index, s)
-      end.
-
-  Definition delete {S} (arr : array S) : ST S unit :=
-    let fix aux (s : arrays) (arr : array S) : arrays :=
-      match arr, s with
-      | _, nil => nil
-      | O, cons x xs => cons nil xs
-      | S n, cons x xs => cons x (aux xs n)
-      end
-    in fun s => (tt, aux s arr).
-End FM.
-
-Module C (E : Element) : Array E.
-  Axiom ST : Type -> Type -> Type.
-  Axiom pure : forall {S A}, A -> ST S A.
-  Axiom bind : forall {S A B}, ST S A -> (A -> ST S B) -> ST S B.
-  Axiom runST : forall {A}, (forall S, ST S A) -> A.
-  Axiom array : Type -> Type.
-  Axiom new : forall {S}, nat -> E.t -> ST S (array S).
-  Axiom set : forall {S}, array S -> nat -> E.t -> ST S unit.
-  Axiom get : forall {S}, array S -> nat -> ST S (option E.t).
-  Axiom delete : forall {S}, array S -> ST S unit.
-End C.
-
-Module Array_Proofs.
-  Module E.
-    Definition t := bool.
-  End E.
-  Module FM := FM E.
-  Module C := C E.
-
-  Definition Rep_nat : Rep nat. Admitted.
-  Definition Rep_t : Rep E.t. Admitted.
-  Axiom Isomorphism_array : forall {S}, Isomorphism (C.array S) (FM.array S).
-  Axiom Isomorphism_ST : forall {S A A'}, Isomorphism A A' -> Isomorphism (C.ST S A) (FM.ST S A').
-
-  Definition pure_ep : extern_properties :=
-    {| type_desc :=
-      @TYPEPARAM (fun (S : Type) `{Rep_S : Rep S} =>
-        @TYPEPARAM (fun (A : Type) `{Rep_A : Rep A} =>
-          @TRANSPARENT A Rep_A (Some (fun arr =>
-            @OPAQUE (C.ST S A) (FM.ST S A) (Isomorphism_ST _) None))))
-     ; prim_fn := @C.pure
-     ; model_fn := @FM.pure
-     ; c_name := "st_pure"
-     |}.
-
-  Definition bind_ep : extern_properties :=
-    {| type_desc :=
-      @TYPEPARAM (fun (S : Type) `{Rep_S : Rep S} =>
-        @TYPEPARAM (fun (A : Type) `{Rep_A : Rep A} =>
-          @TYPEPARAM (fun (B : Type) `{Rep_B : Rep B} =>
-            @OPAQUE (C.ST S A) (FM.ST S A) (Isomorphism_ST _) (Some (fun m =>
-              @OPAQUE (A -> C.ST S B) (A -> FM.ST S B) (Isomorphism_fn _ (Isomorphism_ST _)) (Some (fun f =>
-                @OPAQUE (C.ST S B) (FM.ST S B) (Isomorphism_ST _) None)))))))
-     ; prim_fn := @C.bind
-     ; model_fn := @FM.bind
-     ; c_name := "st_bind"
-     |}.
-
-  Definition runST_ep : extern_properties :=
-    {| type_desc :=
-      @TYPEPARAM (fun (A : Type) `{Rep_A : Rep A} =>
-          @OPAQUE (forall (S : Type), C.ST S A) (forall (S : Type), FM.ST S A)
-                  (@Isomorphism_dep_fn Type Type (fun S => C.ST S A) (fun S => FM.ST S A) _
-                                    (fun s s' m => @Isomorphism_ST _ A A _)) (Some (fun f =>
-            @TRANSPARENT A Rep_A None)))
-     ; prim_fn := @C.runST
-     ; model_fn := @FM.runST
-     ; c_name := "st_runST"
-     |}.
-
-  Definition new_ep : extern_properties :=
-    {| type_desc :=
-      @TYPEPARAM (fun (S : Type) `{Rep_S : Rep S} =>
-        @TRANSPARENT nat Rep_nat (Some (fun n =>
-          @TRANSPARENT E.t Rep_t (Some (fun a =>
-            @OPAQUE (C.ST S (C.array S)) (FM.ST S (FM.array S))
-                    (Isomorphism_ST Isomorphism_array) None)))))
-     ; prim_fn := @C.new
-     ; model_fn := @FM.new
-     ; c_name := "array_new"
-     |}.
-
-  Definition set_ep : extern_properties :=
-    {| type_desc :=
-      @TYPEPARAM (fun (S : Type) `{Rep_S : Rep S} =>
-        @OPAQUE (C.array S) (FM.array S) Isomorphism_array (Some (fun arr =>
-          @TRANSPARENT nat Rep_nat (Some (fun n =>
-            @TRANSPARENT E.t Rep_t (Some (fun a =>
-              @OPAQUE (C.ST S unit) (FM.ST S unit) (Isomorphism_ST _) None)))))))
-     ; prim_fn := @C.set
-     ; model_fn := @FM.set
-     ; c_name := "array_set"
-     |}.
-
-  Definition get_ep : extern_properties :=
-    {| type_desc :=
-      @TYPEPARAM (fun (S : Type) `{Rep_S : Rep S} =>
-        @OPAQUE (C.array S) (FM.array S) Isomorphism_array (Some (fun arr =>
-          @TRANSPARENT nat Rep_nat (Some (fun n =>
-            @OPAQUE (C.ST S (option E.t)) (FM.ST S (option E.t)) (Isomorphism_ST _) None)))))
-     ; prim_fn := @C.get
-     ; model_fn := @FM.get
-     ; c_name := "array_get"
-     |}.
-
-  Definition delete_ep : extern_properties :=
-    {| type_desc :=
-      @TYPEPARAM (fun (S : Type) `{Rep_S : Rep S} =>
-        @OPAQUE (C.array S) (FM.array S) Isomorphism_array (Some (fun arr =>
-          @OPAQUE (C.ST S unit) (FM.ST S unit) (Isomorphism_ST _) None)))
-     ; prim_fn := @C.delete
-     ; model_fn := @FM.delete
-     ; c_name := "array_delete"
-     |}.
-
-  Axiom pure_properties : model_spec pure_ep.
-  Axiom bind_properties : model_spec bind_ep.
-  Axiom runST_properties : model_spec runST_ep.
-  Axiom new_properties : model_spec new_ep.
-  Axiom set_properties : model_spec set_ep.
-  Axiom get_properties : model_spec get_ep.
-  Axiom delete_properties : model_spec delete_ep.
-
-  Ltac prim_rewrites :=
-    repeat eq_refl_match;
-    rewrite ?from_to, ?to_from.
-
-  (* Definition actions_equiv {S A : Type} (x y : FM.ST S A) : Prop := *)
-  (*   forall s, x s = y s. *)
-  (* Set Printing All. *)
-  (* Print actions_equiv. *)
-
-  (* Axiom runST_equiv : forall A (x y : forall (S : Type), FM.ST S A), *)
-  (*     x = y -> *)
-  (*     FM.runST x = FM.runST y. *)
-
-
-  Arguments from A B {_}.
-  Arguments to A B {_}.
-
-  Axiom array_eq : forall S, C.array S = FM.array S.
-  (* Lemma from_eq : *)
-  (*   forall A B x, *)
-  (*     A = B -> *)
-  (*     from A B x = x. *)
-
-  Lemma Isomorphism_FMST {A B : Type} : Isomorphism A B -> Isomorphism (FM.ST unit A) (FM.ST unit B).
-  Proof.
-    intros [f t ft tf].
-    econstructor.
-    Unshelve.
-    3: { intros a x. specialize (a x).
-         exact (f (fst a), (snd a)).}
-    3: { intros a x. specialize (a x).
-         exact (t (fst a), (snd a)).}
-    simpl. intros. apply functional_extensionality. intros. rewrite ?ft, ?tf. destruct (x x0). auto.
-    simpl. intros. apply functional_extensionality. intros. rewrite ?ft, ?tf. destruct (x x0). auto.
-  Defined.
-
-  Lemma from_eq :
-    forall A B x,
-      A = B ->
-      forall (I1 : Isomorphism A B) (I2 : Isomorphism (FM.ST unit B) (FM.ST unit A)),
-        I2 = Isomorphism_sym (Isomorphism_FMST I1) ->
-    (@from A B I1 (fst (@from (FM.ST unit B) (FM.ST unit A) I2 x []))) = fst (x []).
-  Proof.
-    intros A B X eq I1 I2 Ieq.
-    subst.
-  Admitted.
-  (*   unfold fst. *)
-  (*   unfold fst. *)
-  (* Abort. *)
-
-  Lemma set_get :
-    forall {S : Type} (n len : nat) (bound : n < len) (to_set to_fill : E.t),
-      (C.runST (fun _ => C.bind (C.new len to_fill) (fun arr => C.bind (C.set arr n to_set) (fun _ => C.get arr n))))
-        =
-      (C.runST (fun _ => C.pure (Some to_set))).
-  Proof.
-
-    (* Set Printing Implicit. *)
-    (* Unset Printing Notations. *)
-
-
-    intros S n len bound to_set to_fill.
-
-    props runST_properties.
-    prim_rewrites.
-    unfold FM.runST.
-
-    props bind_properties.
-    props pure_properties.
-    props new_properties.
-    unfold FM.bind, FM.pure.
-    prim_rewrites.
-
-    props bind_properties.
-    unfold FM.bind.
-    prim_rewrites.
-
-    props set_properties.
-    prim_rewrites.
-
-    props get_properties.
-    prim_rewrites.
-
-    unfold fst at 4.
-
-    rewrite !to_sym.
-    rewrite !from_trans.
-
-    rewrite from_eq.
-    rewrite !from_sym.
-    3: {
-      unfold Isomorphism_sym.
-      simpl.
-      Set Printing All.
-      Check (@Isomorphism_ST unit (C.array unit) (C.array unit) (@Isomorphism_refl (C.array unit))).
-      Check (@Isomorphism_refl (FM.ST unit (FM.array unit))).
-      replace (@Isomorphism_ST unit (C.array unit) (C.array unit) (@Isomorphism_refl (C.array unit)))
-         with (@Isomorphism_refl (FM.ST unit (FM.array unit))).
-
-    }
-
-
-
-    Set Printing All.
-
-    (* rewrite array_eq. *)
-
-    (* Set Printing Implicit. *)
-
-    unfold FM.new, FM.set, FM.get.
-    unfold repeat.
-
-    simpl.
-    all: try auto.
-
-
-    rewrite !to_sym.
-    rewrite !from_trans.
-
-
-
-    Unset Printing Implicit.
-
-
-    (* rest of the proof is just about the functional model *)
-    Set Printing All.
-    Check (@FM.new unit len to_fill).
-    rewrite ?from_to, ?to_from.
-    unfold FM.new.
-    rewrite ?from_to, ?to_from.
-
-    unfold from.
-
-    assert (forall (x : FM.ST S nat), to (from x) = x).
-    intros. prim_rewrites. auto.
-
-
-    rewrite (H (fun s : FM.arrays => (length s, s ++ [repeat to_fill len]))).
-    rewrite !to_from.
-    unfold FM.get, FM.set, FM.new.
-    simpl.
-    prim_rewrites.
-
-
-  Qed.
-
-
 End Array_Proofs.
 
 End ArrayVerification.
-*)
